theories/Prop/FunctionalInduction.v
@@ -7,7 +7,8 @@
 (**********************************************************************)
 
 Require Import Equations.Tactics.
-Require Import Equations.Prop.Classes Equations.Prop.EqDec Equations.Prop.DepElim.
+Require Import Equations.Prop.Logic
+        Equations.Prop.Classes Equations.Prop.EqDec Equations.Prop.DepElim.
 
 (** The tactic [funind c Hc] applies functional induction on the application 
    [c] which must be of the form [f args] where [f] has a [FunctionalInduction]
@@ -102,8 +103,6 @@ Ltac funelim_sig_tac c tac :=
   (refine (eq_simplification_sigma1 _ _ _ _ _) ||
    refine (eq_simplification_sigma1_nondep_dep _ _ _ _ _) ||
    refine (eq_simplification_sigma1_dep _ _ _ _ _));
-   (* refine (Id_simplification_sigma1_dep _ _ _ _ _) || *)
-   (* refine (Id_simplification_sigma1_nondep_dep _ _ _ _ _)); *)
   let H := fresh "eqargs" in
   let Heq := fresh "Heqcall" in intros H Heq;
   try (rewrite <- Heq; clear Heq); revert_until H; revert H;
@@ -117,8 +116,7 @@ Ltac funelim_sig_tac c tac :=
   unshelve refine_ho elimt; intros;
   cbv beta; simplify_dep_elim; intros_until_block;
   simplify_dep_elim;
-  cbn beta iota delta [eq_rect_dep_r (* Id_rect_r *) eq_rect (* Id_rect *) pack_sigma_eq pack_sigma_eq_nondep
-                                     (* pack_sigma_Id *) (* pack_sigma_Id_nondep *)] in *;
+  cbn beta iota delta [transport eq_elim eq_elim_r eq_rect pack_sigma_eq pack_sigma_eq_nondep] in *;
   simplify_IH_hyps'; (* intros _; *)
   unblock_goal; simplify_IH_hyps; tac c.
 
